Verify right thread in durable message passing

src/examples/durable_mp.v
@@ -6,68 +6,225 @@ From self.high Require Import dprop.
 
 From self.lang Require Import notation lang.
 From self.algebra Require Import view.
-From self.base Require Import primitive_laws class_instances.
+From self.base Require Import primitive_laws class_instances crash_borrow.
 From self.high Require Import proofmode wpc_proofmode.
-From self.high Require Import crash_weakestpre weakestpre recovery_weakestpre.
+From self.high Require Import crash_weakestpre modalities weakestpre recovery_weakestpre
+     protocol crash_borrow.
 
 Section program.
+
   Definition leftProg (x y : loc) : expr :=
-    #x <- #1 ;;
+    #x <- #true ;;
     WB #x ;;
     Fence ;;
-    #y <-{rel} #1.
+    #y <-{rel} #true.
 
   Definition rightProg (y z : loc) : expr :=
-    if: !{acq} #y = #1
-    then Fence ;; #z <- #1
+    if: !{acq} #y = #true
+    then Fence ;; #z <- #true
     else #().
 
   Definition prog (x y z : loc) : expr :=
-    Fork (leftProg x y) ;; rightProg y z.
+    Fork (rightProg y z) ;; leftProg x y.
 
   Definition recovery x z : expr :=
-    if: ! z = #1
-    then assert: ! x = #1
+    if: ! z = #true
+    then assert: ! x = #true
     else #().
+
 End program.
-
-Instance subseteq_nat : SqSubsetEq nat := λ v w, v ≤ w.
-
-Instance subseteq_nat_preorder : PreOrder (⊑@{nat}).
-Proof. apply _. Qed.
-
-Instance nat_abstract_state : AbstractState nat.
-Proof. esplit; apply _. Defined.
 
 Section proof.
   Context `{nvmFixedG Σ, nvmDeltaG Σ}.
 
   Context (x y z : loc).
 
-  Definition inv_x (n : nat) (v : val) (hG : nvmDeltaG Σ) : dProp Σ := ⌜v = #n⌝.
+  Definition inv_x (b : bool) (v : val) (hG : nvmDeltaG Σ) : dProp Σ :=
+    ⌜v = #(Nat.b2n b)⌝.
 
-  Definition inv_y (n : nat) (v : val) (hG : nvmDeltaG Σ) : dProp Σ :=
-    ⌜v = #n⌝ ∗ (⌜n = 1⌝ -∗ know_flush_lb x 1).
+  Program Instance : LocationProtocol inv_x := { bumper n := n }.
+  Next Obligation. iIntros. by iApply post_crash_flush_pure. Qed.
 
-  Definition inv_z (n : nat) (v : val) (hG : nvmDeltaG Σ) : dProp Σ :=
-    ⌜v = #n⌝ ∗ (⌜n = 1⌝ -∗ know_flush_lb x 1).
+  Definition inv_y (b : bool) (v : val) (hG : nvmDeltaG Σ) : dProp Σ :=
+    match b with
+      false => ⌜ v = #false ⌝
+    | true => ⌜ v = #true ⌝ ∗ know_flush_lb x true
+    end.
 
-  Lemma prog_spec k E :
-    {{{
-      ⎡ know_pred x inv_x ⎤ ∗
-      ⎡ know_pred y inv_y ⎤ ∗
-      ⎡ know_pred z inv_z ⎤ ∗
-      x ↦ₚ [0] ∗
-      know_store_lb y 0 ∗
-      z ↦ₚ [0]
-    }}}
-      prog x y z
-    @ k ; E
-    {{{ RET #(); True }}}
-    {{{ <PC> _, ∃ (sx sz : list nat), x ↦ₚ sx ∗ z ↦ₚ sz }}}.
+  Program Instance : LocationProtocol inv_y := { bumper n := n }.
+  Next Obligation.
+    iIntros (? [|] ?); simpl.
+    - iIntros "[% lb]". iCrashFlush. iDestruct "lb" as "(_ & $ & _)". done.
+    - iIntros "%". iApply post_crash_flush_pure. done.
+  Qed.
+
+  Definition inv_z := inv_y.
+  (* Definition inv_z (b : bool) (v : val) (hG : nvmDeltaG Σ) : dProp Σ := *)
+  (*   ⌜v = #(Nat.b2n b)⌝ ∗ (⌜b = true⌝ -∗ know_flush_lb x true). *)
+
+  Definition crash_condition {hD : nvmDeltaG Σ} : dProp Σ :=
+    ∃ (sx sz : list bool),
+      "#xProt" ∷ know_protocol x inv_x ∗
+      "#yProt" ∷ or_lost y (know_protocol y inv_y) ∗
+      "#yShared" ∷ or_lost y (⎡ is_shared_loc y ⎤) ∗
+      "#zProt" ∷ know_protocol z inv_z ∗
+      x ↦ₚ sx ∗
+      z ↦ₚ sz.
+
+  Definition right_crash_condition {hD : nvmDeltaG Σ} : dProp Σ :=
+    ∃ (sz : list bool),
+      "#yProt" ∷ or_lost y (know_protocol y inv_y) ∗
+      "#yShared" ∷ or_lost y (⎡ is_shared_loc y ⎤) ∗
+      "#zProt" ∷ know_protocol z inv_z ∗
+      z ↦ₚ sz.
+
+  (* Lemma crash_condition_impl {hD : nvmDeltaG Σ} (ssX ssZ : list bool) : *)
+  (*   know_protocol x inv_x -∗ know_protocol y inv_y -∗ know_protocol z inv_z -∗ *)
+  (*   x ↦ₚ ssX -∗ *)
+  (*   ⎡ is_shared_loc y ⎤ -∗ *)
+  (*   z ↦ₚ ssZ -∗ *)
+  (*   <PC> hG, crash_condition. *)
+  (* Proof. *)
+  (*   iIntros "xPred yProt zProt xPts yShared zPts". *)
+  (*   iCrash. *)
+  (*   iDestruct "xPts" as (??) "[xPts xRec]". *)
+  (*   iDestruct "zPts" as (??) "[zPts zRec]". *)
+  (*   iExists _, _. *)
+  (*   iDestruct (recovered_at_or_lost with "xRec xPred") as "xPred". *)
+  (*   iDestruct (recovered_at_or_lost with "zRec zProt") as "zProt". *)
+  (*   iFrame. *)
+  (* Qed. *)
+
+  Lemma right_crash_condition_impl {hD : nvmDeltaG Σ} (ssZ : list bool) :
+    know_protocol y inv_y -∗
+    know_protocol z inv_z -∗
+    know_store_lb y false -∗
+    ⎡ is_shared_loc y ⎤ -∗
+    z ↦ₚ ssZ -∗
+    <PC> hD, right_crash_condition.
   Proof.
-    iIntros (Φ Φc).
-    iIntros "(a & b & c)".
+    iIntros "yProt zProt yLb yShared zPts".
+    iCrash.
+    iDestruct "zPts" as (??) "[zPts zRec]".
+    iExists _.
+    iDestruct (recovered_at_or_lost with "zRec zProt") as "zProt".
+    iFrame.
+  Qed.
+
+  (* Prove right crash condition. *)
+  Ltac whack_right_cc :=
+    iSplit;
+    first iApply (right_crash_condition_impl with "yProt zProt yLb yShared zPts").
+
+  Lemma right_prog_spec s k E1 :
+    know_protocol y inv_y -∗
+    know_protocol z inv_z -∗
+    know_store_lb y false -∗
+    ⎡ is_shared_loc y ⎤ -∗
+    z ↦ₚ [false] -∗
+    WPC rightProg y z @ s; k; E1
+    {{ v, z ↦ₚ [false; true] ∨ z ↦ₚ [false] }}
+    {{ <PC> _, right_crash_condition }}.
+  Proof.
+    iIntros "#yProt #zProt #yLb #yShared zPts".
+    (* Evaluate the first load. *)
+    rewrite /rightProg.
+    wpc_bind (!{acq} _)%E.
+    iApply wpc_atomic_no_mask. whack_right_cc.
+    iApply (wp_load_shared _ _ (λ s v, (⌜v = #true⌝ ∗ know_flush_lb x true) ∨ ⌜v = #false⌝)%I inv_y with "[$yProt $yShared $yLb]").
+    { iModIntro. iIntros (?? incl) "a". rewrite /inv_y.
+      destruct s'.
+      - iDestruct "a" as "[% #?]". iFrame "#". naive_solver.
+      - iDestruct "a" as "%". naive_solver. }
+    iNext.
+    iIntros (??) "[yLb' disj]".
+    iDestruct (post_fence_extract _ (⌜v = #true ∨ v = #false⌝)%I with "disj []") as "[disj [-> | ->]]".
+    { iIntros "[[-> _]|->]"; iModIntro; iModIntro; naive_solver. }
+    2: {
+      (* We loaded [false] and this case is trivial. *)
+      whack_right_cc.
+      iModIntro.
+      wpc_pures.
+      { iApply (right_crash_condition_impl with "yProt zProt yLb yShared zPts"). }
+      iModIntro.
+      iRight. iFrame. }
+    (* We loaded [true]. *)
+    whack_right_cc.
+    iModIntro.
+    wpc_pures.
+    { iApply (right_crash_condition_impl with "yProt zProt yLb yShared zPts"). }
+    wpc_bind (Fence).
+    iApply wpc_atomic_no_mask. whack_right_cc.
+    iApply (wp_fence with "disj").
+    iNext.
+    iDestruct 1 as "[[_ #xLb] | %]"; last congruence.
+    whack_right_cc.
+    iModIntro.
+    wpc_pures.
+    { iApply (right_crash_condition_impl with "yProt zProt yLb yShared zPts"). }
+
+    iApply wpc_atomic_no_mask. whack_right_cc.
+    iApply (wp_store_ex _ _ _ _ _ true inv_z with "[$zPts $zProt]").
+    { reflexivity. }
+    { done. }
+    { simpl. iFrame "xLb". done. }
+
+    iIntros "!> zPts /=".
+    whack_right_cc.
+    iModIntro.
+    iLeft. iFrame.
+  Qed.
+
+  Lemma prog_spec k :
+    ⎡ pre_borrow ⎤ ∗
+    know_protocol x inv_x ∗ know_protocol y inv_y ∗ know_protocol z inv_z ∗
+    x ↦ₚ [false] ∗
+    know_store_lb y false ∗
+    ⎡ is_shared_loc y ⎤ ∗
+    z ↦ₚ [false] -∗
+    WPC  prog x y z
+    @ k; ⊤
+    {{ v, True }}
+    {{ <PC> _, crash_condition }}.
+  Proof.
+    iIntros "(pb & #xProt & #yProt & #zProt & xPts & #yLb & #yShared & zPts)".
+    (* iIntros "H". *)
+    rewrite /prog.
+
+    (* We create a crash borrow in order to transfer resources to the forked
+    thread. *)
+    iApply (wpc_crash_borrow_inits _ _ _ _ _ _ (<PC> _, right_crash_condition)%I with "pb [zPts]").
+    { iAccu. }
+    { iModIntro. iIntros "zPts".
+      iDestruct "zProt" as "-#zProt".
+      iDestruct "yProt" as "-#yProt".
+      iDestruct "yShared" as "-#yShared".
+      iCrash.
+      iDestruct "zPts" as (??) "[zPts zRec]".
+      iDestruct (recovered_at_or_lost with "zRec zProt") as "zProt".
+      iExists _. iFrame. }
+    iIntros "cb".
+
+    wpc_bind (Fork _)%E.
+    iApply (wpc_fork with "[cb]").
+    { (* Show safety of the forked off thread. *)
+      iApply (wpc_crash_borrow_open_modify with "cb"); first done.
+      iNext. iSplit; first done.
+      iIntros "zPts". rewrite (left_id True%I (∗)%I).
+
+      iDestruct (right_prog_spec with "yProt zProt yLb yShared zPts") as "wp".
+      iApply (wpc_mono' with "[] [] wp"); last naive_solver.
+      iIntros (?) "[zPts | zPts]".
+      - iExists (z ↦ₚ (_ : list bool)). iFrame.
+        iSplit; last naive_solver.
+        iIntros "!> zPts".
+        iApply (right_crash_condition_impl with "yProt zProt yLb yShared zPts").
+      - iExists (z ↦ₚ (_ : list bool)). iFrame.
+        iSplit; last naive_solver.
+        iIntros "!> zPts".
+        iApply (right_crash_condition_impl with "yProt zProt yLb yShared zPts").
+    }
+    { admit. }
   Abort.
 
 End proof.
